extra/SepROExtra.v
@@ -1,0 +1,71 @@
+
+(* ---------------------------------------------------------------------- *)
+(* ** Extra *)
+
+
+
+Lemma decomposition : forall H,
+  H ==> (\exists H1 H2, \[Normal H1 /\ (haffine H -> haffine H1)]
+                     \* \[ReadOnly H2] \* (H1 \* H2)). 
+Proof using.
+  intros H h K. rewrite (heap_eq_union_rw_ro h).
+  exists (= h^rw) (= h^ro). do 2 rewrite hstar_hpure. splits.
+  { splits. 
+    { intros ? ->. rew_heap*. }
+    { intros F. Transparent haffine. unfolds haffine. intros ? ->.
+      specializes F K. rewrite (heap_eq_union_rw_ro h) in F. 
+      forwards*: heap_affine_union_inv F. } }
+  { intros ? ->. rew_heap*. } 
+  { do 2 esplit. splits*. }
+Qed.
+
+Lemma triple_decomposition : forall t H H' Q,
+  (forall H1 H2, Normal H1 -> ReadOnly H2 -> (haffine H' -> haffine H1) ->
+                 triple t (H \* H1 \* H2) Q) ->
+  triple t (H \* H') Q.
+Proof using.
+  introv M.
+  forwards K: decomposition H'.
+  lets WH: himpl_frame_r H K.
+  applys* triple_conseq WH. 
+  rewrite hstar_comm. (* manual xpull *)
+  rewrite hstar_hexists. applys triple_hexists. intros H1.
+  rewrite hstar_hexists. applys triple_hexists. intros H2.
+  rewrite hstar_assoc. applys triple_hpure. intros (N1&F1).
+  rewrite hstar_assoc. applys triple_hpure. intros N2.
+  rewrite hstar_comm. rewrite <- hstar_assoc.
+  rewrite hstar_assoc. applys* M.
+Qed.
+
+Lemma triple_haffine_pre' : forall t H H' Q,
+  triple t H Q ->
+  haffine H' ->
+  triple t (H \* H') Q.
+Proof using.
+  introv M F. applys triple_decomposition.
+  intros H1 H2 N1 N2 NF. rewrite <- hstar_assoc.
+  applys* triple_frame_ReadOnly.
+  applys* triple_haffine_pre.
+Qed.
+
+
+
+(* not needed, except for next lemma *)
+Lemma hexists_named_eq : forall H,
+  H = (\exists h, \[H h] \* (= h)).
+Proof using.
+  intros. apply himpl_antisym.
+  { intros h K. applys hexists_intro h.
+    rewrite* hstar_hpure_l. }
+  { xpull. intros h K. intros ? ->. auto. }
+Qed.
+
+(* not needed *)
+Lemma triple_named_heap : forall t H Q,
+  (forall h, H h -> triple t (= h) Q) ->
+  triple t H Q.
+Proof using.
+  introv M. rewrite (hexists_named_eq H).
+  applys triple_hexists. intros h.
+  applys* triple_hpure.
+Qed.
